Propagate changes in core DY* repo (#7)
* propagate the pke related renaming from the core DY* repo

* update to new DY* version

* updating flake-lock to newer DY* main

dy-extensions/DY.Simplified.fst
@@ -21,18 +21,18 @@ let start_new_session prin cont =
   set_state prin sid cont;*
   return sid
 
-val pk_enc_for:
+val pke_enc_for:
   #a:Type -> {| parseable_serializeable bytes a |} ->
   principal -> principal ->
   state_id -> string -> 
   a -> 
   traceful (option bytes)
-let pk_enc_for #a alice bob key_sid key_tag plaintext =
-  let*? pk_bob = get_public_key alice key_sid (LongTermPkEncKey key_tag) bob in
-  let* nonce = mk_rand PkNonce (long_term_key_label alice) 32 in
-  return ( Some (pk_enc pk_bob nonce (serialize a plaintext)))
+let pke_enc_for #a alice bob key_sid key_tag plaintext =
+  let*? pk_bob = get_public_key alice key_sid (LongTermPkeKey key_tag) bob in
+  let* nonce = mk_rand PkeNonce (long_term_key_label alice) 32 in
+  return ( Some (pke_enc pk_bob nonce (serialize a plaintext)))
 
-val pk_enc_for_invariant:
+val pke_enc_for_invariant:
   {|protocol_invariants|}->
   tr:trace ->
   #a:Type -> {|parseable_serializeable bytes a|} ->
@@ -45,12 +45,12 @@ val pk_enc_for_invariant:
       trace_invariant tr
   )
   (ensures (
-    let (_, tr_out) = pk_enc_for #a alice bob alice_pki_sid key_tag msg tr in
+    let (_, tr_out) = pke_enc_for #a alice bob alice_pki_sid key_tag msg tr in
     trace_invariant tr_out
   ))
-let pk_enc_for_invariant tr #a alice bob alice_pki_sid key_tag msg = ()
+let pke_enc_for_invariant tr #a alice bob alice_pki_sid key_tag msg = ()
 
-val pk_enc_for_is_publishable:
+val pke_enc_for_is_publishable:
   {|protocol_invariants|} ->
   tr:trace ->
   #a:Type -> {|parseable_serializeable bytes a|} ->
@@ -66,45 +66,45 @@ val pk_enc_for_is_publishable:
     /\ bytes_invariant tr msg_b
     /\ (get_label tr msg_b) `can_flow tr` (long_term_key_label bob)
     /\ (get_label tr msg_b) `can_flow tr` (long_term_key_label alice)
-    /\ (pkenc_pred.pred tr (long_term_key_type_to_usage (LongTermPkEncKey key_tag) bob) msg_b
+    /\ (pke_pred.pred tr (long_term_key_type_to_usage (LongTermPkeKey key_tag) bob) msg_b
       \/ (get_label tr msg_b) `can_flow tr` public
     )
     ))
   (ensures (
-    match pk_enc_for alice bob alice_pki_sid key_tag msg tr with
+    match pke_enc_for alice bob alice_pki_sid key_tag msg tr with
     | (None, _) -> True
     | (Some cipher, tr_out) -> 
         is_publishable tr_out cipher
   ))
-let pk_enc_for_is_publishable tr #a alice bob alice_pki_sid key_tag msg =
-  match pk_enc_for alice bob alice_pki_sid key_tag msg tr with
+let pke_enc_for_is_publishable tr #a alice bob alice_pki_sid key_tag msg =
+  match pke_enc_for alice bob alice_pki_sid key_tag msg tr with
   | (None, _) -> ()
   | (Some cipher, tr_out) -> (
-      let pk_type = LongTermPkEncKey key_tag in
+      let pk_type = LongTermPkeKey key_tag in
       let (Some pk_bob, _) = get_public_key alice alice_pki_sid pk_type bob tr in
-      let (nonce, tr_nonce) = mk_rand PkNonce (long_term_key_label alice) 32 tr in
+      let (nonce, tr_nonce) = mk_rand PkeNonce (long_term_key_label alice) 32 tr in
       let msg = serialize #bytes a msg in
       assert(is_public_key_for tr_out pk_bob pk_type bob);
-      let sk_usg = long_term_key_type_to_usage (LongTermPkEncKey key_tag) bob in
-      introduce pkenc_pred.pred tr sk_usg msg ==> is_publishable tr_out cipher
+      let sk_usg = long_term_key_type_to_usage (LongTermPkeKey key_tag) bob in
+      introduce pke_pred.pred tr sk_usg msg ==> is_publishable tr_out cipher
       with _ .
-        pkenc_pred.pred_later tr tr_nonce sk_usg msg;
+        pke_pred.pred_later tr tr_nonce sk_usg msg;
       ()
 )  
 
-val pk_dec_with_key_lookup:
+val pke_dec_with_key_lookup:
   #a:Type -> {| parseable_serializeable bytes a |} ->
   principal -> 
   state_id -> string ->
   bytes ->
   traceful (option a)
-let pk_dec_with_key_lookup #a prin keys_sid key_tag cipher =
-  let*? sk_a = get_private_key prin keys_sid (LongTermPkEncKey key_tag) in
-  let*? plaintext = return (pk_dec sk_a cipher) in 
+let pke_dec_with_key_lookup #a prin keys_sid key_tag cipher =
+  let*? sk_a = get_private_key prin keys_sid (LongTermPkeKey key_tag) in
+  let*? plaintext = return (pke_dec sk_a cipher) in 
   // guard_tr ( Some? (parse a plaintext));*?
   return (parse a plaintext)
 
-val bytes_invariant_pk_dec_with_key_lookup:
+val bytes_invariant_pke_dec_with_key_lookup:
   {|protocol_invariants|} ->
   tr:trace ->
   #a:Type -> {|parseable_serializeable bytes a|} ->
@@ -117,28 +117,28 @@ val bytes_invariant_pk_dec_with_key_lookup:
     /\ bytes_invariant tr cipher
   ))
   (ensures(
-    match pk_dec_with_key_lookup #a alice keys_sid key_tag cipher tr with
+    match pke_dec_with_key_lookup #a alice keys_sid key_tag cipher tr with
     | (None, _) -> True
     | (Some plaintext, _) -> (
         let plain_b = serialize #bytes a plaintext in
         is_knowable_by (long_term_key_label alice ) tr plain_b /\
-      ( let sk_usg = (long_term_key_type_to_usage (LongTermPkEncKey key_tag) alice) in
+      ( let sk_usg = (long_term_key_type_to_usage (LongTermPkeKey key_tag) alice) in
         ((
           //PkKey? sk_usg /\
-          pkenc_pred.pred tr sk_usg plain_b )
+          pke_pred.pred tr sk_usg plain_b )
           \/ (
           (get_label tr plain_b `can_flow tr` public)
         )
       )
     )
   )))
-let bytes_invariant_pk_dec_with_key_lookup tr #a alice keys_sid key_tag cipher = 
-  match pk_dec_with_key_lookup #a alice keys_sid key_tag cipher tr with
+let bytes_invariant_pke_dec_with_key_lookup tr #a alice keys_sid key_tag cipher = 
+  match pke_dec_with_key_lookup #a alice keys_sid key_tag cipher tr with
   | (None, _) -> ()
   | (Some plaintext, _) -> (
-      let (Some sk_alice, _) = get_private_key alice keys_sid (LongTermPkEncKey key_tag) tr in
-      let Some cipher_dec = pk_dec sk_alice cipher in 
-       let sk_usg = (long_term_key_type_to_usage (LongTermPkEncKey key_tag) alice) in
-      bytes_invariant_pk_dec tr sk_alice sk_usg cipher;
+      let (Some sk_alice, _) = get_private_key alice keys_sid (LongTermPkeKey key_tag) tr in
+      let Some cipher_dec = pke_dec sk_alice cipher in 
+       let sk_usg = (long_term_key_type_to_usage (LongTermPkeKey key_tag) alice) in
+      bytes_invariant_pke_dec tr sk_alice sk_usg cipher;
       serialize_parse_inv_lemma a cipher_dec
   )
