examples/nsl_pk_no_events_lookup/DY.Example.NSL.Protocol.Stateful.Proof.fst
@@ -168,10 +168,10 @@ let send_msg1_proof tr global_sess_id alice sess_id =
   match get_state alice sess_id tr with
   | (Some (InitiatorSendingMsg1 bob n_a), tr) -> (
       assert(state_was_set_some_id tr alice (InitiatorSendingMsg1 bob n_a));
-    match get_public_key alice global_sess_id.pki (LongTermPkEncKey "NSL.PublicKey") bob tr with
+    match get_public_key alice global_sess_id.pki (LongTermPkeKey "NSL.PublicKey") bob tr with
     | (None, tr) -> ()
     | (Some pk_b, tr) -> (
-      let (nonce, tr) = mk_rand PkNonce (long_term_key_label alice) 32 tr in
+      let (nonce, tr) = mk_rand PkeNonce (long_term_key_label alice) 32 tr in
       compute_message1_proof tr alice bob pk_b n_a nonce
     )
   )
@@ -195,11 +195,11 @@ let send_msg1__proof tr global_sess_id alice bob =
   set_state_state_was_set alice sess_id st tr;
   assert(state_was_set_some_id tr_state alice (InitiatorSendingMsg1 bob n_a));
 
-  match get_public_key alice global_sess_id.pki (LongTermPkEncKey "NSL.PublicKey") bob tr_state with
+  match get_public_key alice global_sess_id.pki (LongTermPkeKey "NSL.PublicKey") bob tr_state with
     | (None, tr) -> ()
     | (Some pk_b, tr) -> (
     
-      let (nonce, tr) = mk_rand PkNonce (long_term_key_label alice) 32 tr in
+      let (nonce, tr) = mk_rand PkeNonce (long_term_key_label alice) 32 tr in
       compute_message1_proof tr alice bob pk_b n_a nonce;
       
   ()
@@ -218,7 +218,7 @@ let prepare_msg2_proof tr global_sess_id bob msg_id =
   match recv_msg msg_id tr with
   | (None, tr) -> ()
   | (Some msg, tr) -> (
-    match get_private_key bob global_sess_id.private_keys (LongTermPkEncKey "NSL.PublicKey") tr with
+    match get_private_key bob global_sess_id.private_keys (LongTermPkeKey "NSL.PublicKey") tr with
     | (None, tr) -> ()
     | (Some sk_b, tr) -> (
       decode_message1_proof tr bob msg sk_b
@@ -238,10 +238,10 @@ let send_msg2_proof tr global_sess_id bob sess_id =
   match get_state bob sess_id tr with
   | (Some (ResponderSendingMsg2 alice n_a n_b), tr) -> (
     assert(state_was_set_some_id tr bob (ResponderSendingMsg2 alice n_a n_b));
-    match get_public_key bob global_sess_id.pki (LongTermPkEncKey "NSL.PublicKey") alice tr with
+    match get_public_key bob global_sess_id.pki (LongTermPkeKey "NSL.PublicKey") alice tr with
     | (None, tr) -> ()
     | (Some pk_a, tr) -> (
-      let (nonce, tr) = mk_rand PkNonce (long_term_key_label bob) 32 tr in
+      let (nonce, tr) = mk_rand PkeNonce (long_term_key_label bob) 32 tr in
       compute_message2_proof tr bob {n_a; alice;} pk_a n_b nonce
     )
   )
@@ -260,7 +260,7 @@ let send_msg2__proof tr global_sess_id bob msg_id =
   match recv_msg msg_id tr with
   | (None, tr) -> ()
   | (Some msg, tr) -> (
-    match get_private_key bob global_sess_id.private_keys (LongTermPkEncKey "NSL.PublicKey") tr with
+    match get_private_key bob global_sess_id.private_keys (LongTermPkeKey "NSL.PublicKey") tr with
     | (None, tr) -> ()
     | (Some sk_b, tr) -> (
       decode_message1_proof tr bob msg sk_b;
@@ -276,10 +276,10 @@ let send_msg2__proof tr global_sess_id bob msg_id =
     let (_, tr_st) = set_state bob sess_id st tr in
 //    set_state_state_was_set bob sess_id st tr_st;
     assert(state_was_set_some_id tr_st bob st);
-    match get_public_key bob global_sess_id.pki (LongTermPkEncKey "NSL.PublicKey") alice tr_st with
+    match get_public_key bob global_sess_id.pki (LongTermPkeKey "NSL.PublicKey") alice tr_st with
     | (None, tr) -> ()
     | (Some pk_a, tr) -> (
-      let (nonce, tr) = mk_rand PkNonce (long_term_key_label bob) 32 tr in
+      let (nonce, tr) = mk_rand PkeNonce (long_term_key_label bob) 32 tr in
       compute_message2_proof tr bob {n_a; alice;} pk_a n_b nonce
     )
   ))
@@ -298,7 +298,7 @@ let prepare_msg3_proof tr global_sess_id alice sess_id msg_id =
   match recv_msg msg_id tr with
   | (None, tr) -> ()
   | (Some msg, tr) -> (
-    match get_private_key alice global_sess_id.private_keys (LongTermPkEncKey "NSL.PublicKey") tr with
+    match get_private_key alice global_sess_id.private_keys (LongTermPkeKey "NSL.PublicKey") tr with
     | (None, tr) -> ()
     | (Some sk_a, tr) -> (
       match get_state alice sess_id tr with
@@ -322,7 +322,7 @@ let prepare_msg3__proof tr global_sess_id alice msg_id =
   match recv_msg msg_id tr with
   | (None, tr) -> ()
   | (Some msg, tr) -> (
-    match get_private_key alice global_sess_id.private_keys (LongTermPkEncKey "NSL.PublicKey") tr with
+    match get_private_key alice global_sess_id.private_keys (LongTermPkeKey "NSL.PublicKey") tr with
     | (None, tr) -> ()
     | (Some sk_a, tr) -> (
         match decode_message2_ alice msg sk_a with
@@ -354,10 +354,10 @@ let send_msg3_proof tr global_sess_id alice sess_id =
   match get_state alice sess_id tr with
   | (Some (InitiatorSendingMsg3 bob n_a n_b), tr) -> (
     assert(state_was_set_some_id tr alice (InitiatorSendingMsg3 bob n_a n_b));
-    match get_public_key alice global_sess_id.pki (LongTermPkEncKey "NSL.PublicKey") bob tr with
+    match get_public_key alice global_sess_id.pki (LongTermPkeKey "NSL.PublicKey") bob tr with
     | (None, tr) -> ()
     | (Some pk_b, tr) -> (
-      let (nonce, tr) = mk_rand PkNonce (long_term_key_label alice) 32 tr in
+      let (nonce, tr) = mk_rand PkeNonce (long_term_key_label alice) 32 tr in
       compute_message3_proof tr alice bob pk_b n_b nonce
     )
   )
@@ -378,7 +378,7 @@ let send_msg3__proof tr global_sess_id alice msg_id =
     match recv_msg msg_id tr with
   | (None, tr) -> ()
   | (Some msg, tr) -> (
-    match get_private_key alice global_sess_id.private_keys (LongTermPkEncKey "NSL.PublicKey") tr with
+    match get_private_key alice global_sess_id.private_keys (LongTermPkeKey "NSL.PublicKey") tr with
     | (None, tr) -> ()
     | (Some sk_a, tr) -> (
         match decode_message2_ alice msg sk_a with
@@ -397,10 +397,10 @@ let send_msg3__proof tr global_sess_id alice msg_id =
         let new_st = InitiatorSendingMsg3 bob n_a n_b in
         let (_, tr_state) = set_state alice sid new_st tr in
         assert(state_was_set_some_id tr_state alice new_st);
-    match get_public_key alice global_sess_id.pki (LongTermPkEncKey "NSL.PublicKey") bob tr_state with
+    match get_public_key alice global_sess_id.pki (LongTermPkeKey "NSL.PublicKey") bob tr_state with
     | (None, tr) -> ()
     | (Some pk_b, tr) -> (
-      let (nonce, tr) = mk_rand PkNonce (long_term_key_label alice) 32 tr in
+      let (nonce, tr) = mk_rand PkeNonce (long_term_key_label alice) 32 tr in
       compute_message3_proof tr alice bob pk_b n_b nonce
     )
   ))
@@ -436,7 +436,7 @@ let receive_msg3_proof tr global_sess_id bob sess_id msg_id =
   match recv_msg msg_id tr with
   | (None, tr) -> ()
   | (Some msg, tr) -> (
-    match get_private_key bob global_sess_id.private_keys (LongTermPkEncKey "NSL.PublicKey") tr with
+    match get_private_key bob global_sess_id.private_keys (LongTermPkeKey "NSL.PublicKey") tr with
     | (None, tr) -> ()
     | (Some sk_b, tr) -> (
         match decode_message3_ msg sk_b with
