examples/Online_with_secrecy_both/DY.OnlineSB.Run.fst
@@ -17,11 +17,11 @@ let run () : traceful (option unit ) =
 
   // Generate private key for Alice
   let* alice_global_session_priv_key_id = initialize_private_keys alice in
-  generate_private_key alice alice_global_session_priv_key_id (LongTermPkEncKey key_tag);*
+  generate_private_key alice alice_global_session_priv_key_id (LongTermPkeKey key_tag);*
   
   // Generate private key for Bob
   let* bob_global_session_priv_key_id = initialize_private_keys bob in
-  generate_private_key bob bob_global_session_priv_key_id (LongTermPkEncKey key_tag);*
+  generate_private_key bob bob_global_session_priv_key_id (LongTermPkeKey key_tag);*
 
   // Store Bob's public key in Alice's state
   // 1. Initialize Alice's session to store public keys
@@ -29,15 +29,15 @@ let run () : traceful (option unit ) =
   // 3. Compute the public key from the private key
   // 4. Install Bob's public key in Alice's public key store
   let* alice_global_session_pub_key_id = initialize_pki alice in
-  let*? priv_key_bob = get_private_key bob bob_global_session_priv_key_id (LongTermPkEncKey key_tag) in
+  let*? priv_key_bob = get_private_key bob bob_global_session_priv_key_id (LongTermPkeKey key_tag) in
   let pub_key_bob = pk priv_key_bob in
-  install_public_key alice alice_global_session_pub_key_id (LongTermPkEncKey key_tag) bob pub_key_bob;*
+  install_public_key alice alice_global_session_pub_key_id (LongTermPkeKey key_tag) bob pub_key_bob;*
 
   // Store Alice's public key in Bob's state
   let* bob_global_session_pub_key_id = initialize_pki bob in
-  let*? priv_key_alice = get_private_key alice alice_global_session_priv_key_id (LongTermPkEncKey key_tag) in
+  let*? priv_key_alice = get_private_key alice alice_global_session_priv_key_id (LongTermPkeKey key_tag) in
   let pub_key_alice = pk priv_key_alice in
-  install_public_key bob bob_global_session_pub_key_id (LongTermPkEncKey key_tag) alice pub_key_alice;*
+  install_public_key bob bob_global_session_pub_key_id (LongTermPkeKey key_tag) alice pub_key_alice;*
 
   let alice_global_session_ids: global_sess_ids = {pki=alice_global_session_pub_key_id; private_keys=alice_global_session_priv_key_id} in
   let bob_global_session_ids: global_sess_ids = {pki=bob_global_session_pub_key_id; private_keys=bob_global_session_priv_key_id} in
